model/Bijection.v
@@ -1,0 +1,118 @@
+Definition Bijection (A:Set) (B:Set) :=
+  { fg : (A->B)*(B->A) |
+    (forall (a:A),
+       (snd fg) ((fst fg) a) = a)
+    /\
+    (forall (b:B),
+       (fst fg) ((snd fg) b) = b) }.
+
+Definition biject_to {A} {B} (bi:Bijection A B) (a:A) : B :=
+  (fst (proj1_sig bi)) a.
+Definition biject_from {A} {B} (bi:Bijection A B) (b:B) : A :=
+  (snd (proj1_sig bi)) b.
+
+Definition Bijects {A:Set} {B:Set} (bi:Bijection A B) (a:A) (b:B) :=
+  biject_to bi a = b
+  /\ biject_from bi b = a.
+
+Lemma Bijects_fun_right:
+  forall A B (b:Bijection A B) x y1 y2,
+    Bijects b x y1 ->
+    Bijects b x y2 ->
+    y1 = y2.
+Proof.
+  intros A B b x y1 y2.
+  intros [B1_l B1_r] [B2_l B2_r].
+  congruence.
+Qed.
+
+Lemma Bijects_fun_left:
+  forall A B (b:Bijection A B) x1 x2 y,
+    Bijects b x1 y ->
+    Bijects b x2 y ->
+    x1 = x2.
+Proof.
+  intros A B b x1 x2 y.
+  intros [B1_l B1_r] [B2_l B2_r].
+  congruence.
+Qed.
+
+Definition Bijects_to_dec :
+  forall A B (bi:Bijection A B) a,
+    { b | Bijects bi a b }.
+Proof.
+  intros. exists (biject_to bi a).
+  unfold Bijects. intuition.
+  unfold biject_from, biject_to.
+  destruct bi as [[f g] [F G]].
+  simpl in *. auto.
+Defined.
+
+Definition Bijects_from_dec :
+  forall {A B} (bi:Bijection A B) b,
+    { a | Bijects bi a b }.
+Proof.
+  intros. exists (biject_from bi b).
+  unfold Bijects. intuition.
+  unfold biject_from, biject_to.
+  destruct bi as [[f g] [F G]].
+  simpl in *. auto.
+Defined.
+
+Ltac rewrite_biject_funr :=
+  match goal with
+    | [ H1: Bijects ?b ?x _, H2: Bijects ?b ?x _ |- _ ] =>
+      erewrite (Bijects_fun_right _ _ _ _ _ _ H1 H2) in *; clear H1 H2
+  end.
+
+(* rewrite_biject_funr tests *)
+Goal forall tin tout (b: Bijection tin tout) x v1 v2,
+       Bijects b x v1 -> Bijects b x v2 -> v1 = v2.
+intros; rewrite_biject_funr; trivial.
+Qed.
+
+Goal forall tin tout (b: Bijection tin tout) x v1 v2, Bijects b x v1 -> Bijects b x v2 -> v1 <> v2 -> False.
+intros; rewrite_biject_funr; intuition.
+Qed.
+
+Section BijExamples.
+  Require Import Typ Util.
+  Require Import Coq.Arith.Arith_base.
+  Definition SwapCons {A B} (p : A * B) :=
+    match p with | (x, y) => (y, x) end.
+  
+  Definition SwapConsBij {A B : Set} : Bijection (A * B) (B * A).
+    refine ({{ (SwapCons, SwapCons )}}); split; intros p; destruct p; reflexivity.
+  Defined.
+
+  Definition SwapWithZero n m :=
+    if eq_nat_dec m 0
+    then n
+    else if eq_nat_dec m n
+         then 0
+         else m.
+  
+  Lemma SwapWithZero_Swaps : forall n a, (SwapWithZero n) ((SwapWithZero n) a) = a.
+  Proof.
+    intros n n0.
+    unfold SwapWithZero.
+    destruct (eq_nat_dec n0 0); subst; auto.
+    destruct (eq_nat_dec n 0); auto.
+    destruct (eq_nat_dec n n); subst; auto.
+    intuition.
+    destruct (eq_nat_dec n0 n).
+    destruct (eq_nat_dec 0 0); subst; auto.
+    intuition.
+    destruct (eq_nat_dec n0 0); subst; auto.
+    intuition.
+    destruct (eq_nat_dec n0 n); subst.
+    intuition.
+    auto.
+  Qed.
+
+  Definition SwapWithZeroBijection (n: nat) : Bijection (tdenote TNat) (tdenote TNat).
+    simpl.
+    refine ({{(SwapWithZero n, SwapWithZero n)}}).
+    split; apply SwapWithZero_Swaps.
+  Defined.
+End BijExamples.
