model/Fairness.v
@@ -1,0 +1,495 @@
+Require Import Coq.Arith.Arith_base.
+Require Import Coq.Numbers.Natural.Peano.NPeano.
+Require Import Coq.Arith.Div2 Coq.Arith.Even.
+Require Import Coq.Lists.ListSet.
+
+Require Import Enum Pairing Sets Trace Typ Util.
+
+Definition Fair2 {tout} (k : forall {ty1 ty2}, Enum ty1 -> Enum ty2 -> Enum (tout ty1 ty2)) :=
+  forall n,
+  exists equilibrium,
+    match Trace_lt (k (E_Trace zero E_Nat) (E_Trace one E_Nat)) equilibrium with
+      | Tracing l_uses r_uses _ _ =>
+        n < equilibrium /\ l_uses ≃ r_uses
+    end.
+
+Definition Fair3 {tout} (k : forall {ty1 ty2 ty3}, Enum ty1 -> Enum ty2 -> Enum ty3 -> Enum (tout ty1 ty2 ty3)) :=
+  forall n,
+  exists equilibrium,
+    match Trace_lt (k (E_Trace zero E_Nat) (E_Trace one E_Nat) (E_Trace two E_Nat)) equilibrium with
+      | Tracing z_uses o_uses t_uses _ =>
+        n < equilibrium /\ z_uses ≃ o_uses /\ o_uses ≃ t_uses
+    end.
+
+(* Definition Fair4 (k : Enum -> Enum -> Enum -> Enum -> Enum) := *)
+(*   forall n, *)
+(*   exists equilibrium, *)
+(*     match Trace_lt (k (E_Trace zero E_Nat) (E_Trace one E_Nat) (E_Trace two E_Nat) (E_Trace three E_Nat)) equilibrium with *)
+(*       | Tracing z_uses o_uses tw_uses th_uses => *)
+(*         n < equilibrium /\ z_uses ≃ o_uses /\ o_uses ≃ tw_uses /\ tw_uses ≃ th_uses *)
+(*     end. *)
+
+Definition AltUnfair3 {tout} (k : forall {ty1 ty2 ty3}, Enum ty1 -> Enum ty2 -> Enum ty3 -> Enum (tout ty1 ty2 ty3)) :=
+  exists threshold,
+    forall eq_cand,
+      eq_cand > threshold ->
+      match Trace_lt (k (E_Trace zero E_Nat) (E_Trace one E_Nat) (E_Trace two E_Nat)) eq_cand with
+        | Tracing use0 use1 use2 _ =>
+          (~ (use0 ≃ use1)) \/ (~ (use1 ≃ use2)) \/ (~ (use0 ≃ use2))
+      end.
+
+Theorem AltUnfair3Suff {tout} (k : forall {ty1 ty2 ty3}, Enum ty1 -> Enum ty2 -> Enum ty3 -> Enum (tout ty1 ty2 ty3)) : AltUnfair3 (@k) -> ~ (Fair3 (@k)).
+Proof.
+  unfold AltUnfair3, Fair3, not.
+  intros [thresh Halt] Hunf.
+  destruct (Hunf thresh) as [eq_cand Hblah].
+  clear Hunf.
+  remember (Halt eq_cand).
+  clear Halt Heqy.
+  destruct (Trace_lt (k _ _ _ (E_Trace zero E_Nat) (E_Trace one E_Nat) (E_Trace two E_Nat))
+                     eq_cand) as [t0 t1 t2 t3] in *.
+  intuition.
+  assert (t0 ≃ t2) by (eapply set_eq_trans; eauto); contradiction.
+Qed.
+
+Section SumFair.
+  Lemma Sum_precise
+  : forall {tyl tyr} n (e1: Enum tyl) (e2: Enum tyr),
+      Trace_lt (E_Sum e1 e2) (double n) ≡ (Trace_lt e1 n) ⊔ (Trace_lt e2 n).
+  Proof.
+    intros; induction n; [compute; tauto|];
+    rewrite double_S; unfold Trace_lt at 1; fold (@Trace_lt (TSum tyl tyr)); unfold Trace_on;
+    remember (Enumerates_from_dec (E_Sum e1 e2) (S (double n))) as Er; destruct Er as [[vr tr] Er];
+    remember (Enumerates_from_dec (E_Sum e1 e2) (double n)) as El; destruct El as [[vl tl] El]; simpl;
+    eapply trace_eq_trans; [apply trace_plus_assoc|];
+    eapply trace_eq_trans; [apply trace_plus_cong; [apply trace_plus_comm | apply trace_eq_refl]|];
+    eapply trace_eq_trans; [apply trace_eq_symm; apply trace_plus_assoc|];
+    eapply trace_eq_trans; [apply trace_plus_cong; [apply trace_eq_refl|]; apply trace_plus_cong; [apply trace_eq_refl|]; apply IHn |];
+    eapply trace_eq_trans; [apply trace_plus_cong; [apply trace_eq_refl| apply trace_plus_assoc]|];
+    eapply trace_eq_trans; [apply trace_plus_cong; [apply trace_eq_refl| apply trace_plus_cong; [apply trace_plus_comm | apply trace_eq_refl]]|];
+    eapply trace_eq_trans; [apply trace_plus_cong; [apply trace_eq_refl|apply trace_eq_symm; apply trace_plus_assoc ]|];
+    eapply trace_eq_trans; [apply trace_plus_assoc|];
+    apply trace_plus_cong; apply trace_plus_cong; [| apply trace_eq_refl | | apply trace_eq_refl];
+    [ unfold Trace_on; destruct (Enumerates_from_dec e1 n) as [[x' t'] Henum']; simpl;
+      clear HeqEr; clear dependent vr; clear tr HeqEl;
+      invert_Enumerates; subst; even_odd_crush; subst; Eff; subst; apply trace_eq_refl
+    | clear HeqEr HeqEl; unfold Trace_on;
+      destruct (Enumerates_from_dec e2 n) as [[x' t'] Henum']; simpl;
+      invert_Enumerates; subst; even_odd_crush; repeat subst;
+      Eff; subst; apply trace_eq_refl
+    ].
+  Qed.
+
+  (* Proof idea: equilibrium = 2 * n + 2,  uses = 0..(S n) *)
+  Theorem SumFair : Fair2 (@E_Sum).
+  Proof.
+    unfold Fair2.
+    intros n.
+    exists (double (S n)).
+    remember (Trace_lt (E_Sum (E_Trace zero E_Nat) (E_Trace one E_Nat)) (double (S n))) as t; destruct t as [tz to ttw tth].
+    split; [unfold double; nliamega| ].
+
+    remember (Sum_precise (S n) (E_Trace zero E_Nat) (E_Trace one E_Nat)).
+    apply set_eq_trans with (z_to_n (S n));
+      [ replace tz with (trace_proj zero (Tracing tz to ttw tth)) by trivial
+      | replace to with (trace_proj one (Tracing tz to ttw tth)) by trivial; apply set_eq_symm
+      ];
+      (eapply set_eq_trans; [apply trace_eq_proj; rewrite Heqt; eassumption|]).
+    rewrite trace_proj_plus_distrl; rewrite (trace_lt_Nat_off _ zero one); [| discriminate].
+    eapply set_eq_trans; [apply set_union_unitr | apply set_eq_symm; apply trace_lt_Nat].
+
+    rewrite trace_proj_plus_distrl; rewrite (trace_lt_Nat_off _ one zero); [| discriminate].
+    eapply set_eq_trans; [apply set_union_unitl | apply set_eq_symm; apply trace_lt_Nat].
+  Qed.
+End SumFair.
+
+Section NaiveSum3Unfair.
+  Definition NaiveSum3 {ty1 ty2 ty3} (e1: Enum ty1) (e2: Enum ty2) (e3: Enum ty3) :=
+    E_Sum e1 (E_Sum e2 e3).
+
+  Notation x4 n := (double (double n)).
+  
+  Lemma par4 : forall n, (n = x4 (div2 (div2 n)) /\ even n /\ even (div2 n))
+                         \/ (n = (x4 (div2 (div2 n))) + 1 /\ odd n /\ even (div2 n))
+                         \/ (n = (x4 (div2 (div2 n))) + 2 /\ even n /\ odd (div2 n))
+                         \/ (n = (x4 (div2 (div2 n))) + 3 /\ odd n /\ odd (div2 n)).
+  Proof.
+    intros.
+    destruct (even_odd_dec n).
+    - remember (even_div2 n e).
+      destruct (even_odd_dec (div2 n)).
+      + left; split; [| split]; try assumption.
+        rewrite <-even_double by assumption.
+        apply even_double; assumption.
+      + right; right; left; split; [| split]; try assumption.
+        replace (double (double (div2 (div2 n))) + 2) with (S (S (double (double (div2 (div2 n)))))) by nliamega.
+        rewrite <-double_S.
+        rewrite <-odd_double by assumption.
+        apply even_double; assumption.
+    - destruct (even_odd_dec (div2 n)).
+      + right; left; split; [| split]; try assumption.
+        rewrite <-even_double by assumption.
+        replace (double (div2 n) + 1) with (S (double (div2 n))) by nliamega.
+        apply odd_double; assumption.
+      + right; right; right; split; [| split]; try assumption.
+        replace (double (double (div2 (div2 n))) + 3) with (S (S (S (double (double (div2 (div2 n))))))) by nliamega.
+        rewrite <-double_S.
+        rewrite <-odd_double by assumption.
+        apply odd_double; assumption.
+  Qed.
+
+  Lemma div4big : forall n, n >= 8 -> (div2 (div2 n) >= 2).
+  Proof.
+    intros n ?; remember (n - 8) as k; replace n with (8 + k); simpl; nliamega.
+  Qed.
+
+  Lemma div2div4 : forall n, n >= 8 -> exists m p, 2 * m <= n < 4 * p /\ p < m.
+  Proof.
+    intros n Hn4.
+    remember (S (div2 (S (div2 n)))) as p.
+    remember (S p) as m.
+    exists m.
+    exists p.
+    split; [| nliamega].
+    subst.
+    replace (4 * _) with (2 * (2 * (S (div2 (S (div2 n)))))) by nliamega.
+    assert (div2 (div2 n) >= 2) by (apply div4big; assumption).
+    repeat (rewrite <-double_twice).
+    destruct (par4 n) as [[Hpar [? ?]] | [[Hpar [? ?]] | [[Hpar [? ?]] | [Hpar [? ?]]]]]; rewrite Hpar at 2; rewrite Hpar at 3.
+    - clear H0; split.
+      + rewrite double_twice; rewrite double_twice.
+        apply mult_le_compat_l.
+        rewrite <-even_div2 by assumption.
+        unfold double.
+        nliamega.
+      + rewrite <-even_div2 by assumption.
+        (repeat (rewrite double_twice)).
+        nliamega.
+    - split.
+      + rewrite double_S.
+        replace (double (double (div2 (div2 n))) + 1 ) with (S (double (double (div2 (div2 n))))) by nliamega.
+        apply le_n_S.
+        rewrite <-even_div2 by assumption.
+        unfold double.
+        nliamega.
+      + rewrite <-even_div2 by assumption.
+        replace (_ + 1) with (S (double (double (div2 (div2 n))))) by nliamega.
+        unfold double; nliamega.
+    - split.
+      + rewrite double_S.
+        rewrite double_S.
+        rewrite <-odd_div2 by assumption.
+        rewrite double_S.
+        replace (double (double (div2 (div2 n))) + 2) with (S (S (double (double (div2 (div2 n)))))) by nliamega.
+        repeat apply le_n_S.
+        unfold double; nliamega.
+      + rewrite <-odd_div2 by assumption.
+        repeat rewrite double_S.
+        nliamega.
+    - split.
+      + rewrite double_S.
+        rewrite double_S.
+        rewrite <-odd_div2 by assumption.
+        rewrite double_S.
+        replace (double (double (div2 (div2 n))) + 2) with (S (S (double (double (div2 (div2 n)))))) by nliamega.
+        repeat apply le_n_S.
+        unfold double; nliamega.
+      + rewrite <-odd_div2 by assumption.
+        repeat rewrite double_S.
+        nliamega.
+  Qed.
+
+  Lemma SumSum_precise
+  : forall n {ty1 ty2 ty3} (e1: Enum ty1) (e2: Enum ty2) (e3: Enum ty3),
+      Trace_lt (E_Sum e1 (E_Sum e2 e3)) (double (double n))
+      ≡ (Trace_lt e1 (double n)) ⊔ ((Trace_lt e2 n) ⊔ (Trace_lt e3 n)).
+  Proof.
+    intros.
+    eapply trace_eq_trans; [apply Sum_precise|].
+    apply trace_plus_cong; [apply trace_eq_refl|].
+    apply Sum_precise.
+  Qed.
+
+  Definition NS3T := NaiveSum3 (E_Trace zero E_Nat)
+                               (E_Trace one  E_Nat)
+                               (E_Trace two  E_Nat).
+
+  Lemma NS3Tl_precise
+  : forall n,
+      (trace_proj zero (Trace_lt NS3T (double n))) ≃ (z_to_n n).
+  Proof.
+    intros n.
+    eapply set_eq_trans; [apply trace_eq_proj; apply Sum_precise|].
+    rewrite trace_proj_plus_distrl.
+    eapply set_eq_trans; [| apply set_union_unitr].
+    apply set_union_cong.
+    apply set_eq_symm; apply trace_lt_Nat.
+    rewrite trace_lt_Sum_off; [apply set_eq_refl| | ]; (intros; rewrite trace_off; [trivial | discriminate ]).
+  Qed.
+
+  Lemma NS3Tr_precise
+  : forall n,
+      (trace_proj one (Trace_lt NS3T (double (double n)))) ≃ z_to_n n.
+  Proof.
+    intros n.
+    eapply set_eq_trans; [apply trace_eq_proj; apply SumSum_precise|].
+    eapply set_eq_trans; [apply trace_eq_proj; apply trace_plus_comm|].
+    eapply set_eq_trans; [apply trace_eq_proj; apply trace_eq_symm; apply trace_plus_assoc|].
+    rewrite trace_proj_plus_distrl.
+    eapply set_eq_trans; [| apply set_union_unitr].
+    apply set_union_cong; [apply set_eq_symm; apply trace_lt_Nat|].
+    rewrite trace_proj_plus_distrl.
+    repeat (rewrite trace_lt_Nat_off; [| discriminate]).
+    compute; tauto.
+  Qed.
+
+  Theorem NaiveSum3Unfair : ~ (Fair3 (@NaiveSum3)).
+  Proof.
+    apply AltUnfair3Suff; unfold AltUnfair3; fold NS3T.
+    exists 7.
+    intros n H.
+    remember (Trace_lt NS3T n) as t; destruct t as [s0 s1 s2 s4].
+    assert (exists m p, 2 * m <= n < 4 * p /\ p < m) as [m [p [[Hmn Hnp] Hpn]]] by (apply div2div4; nliamega).
+    left.
+    
+    assert (~ s0 ⊂ s1); [| intros [? ?]; contradiction ].
+
+    assert ((z_to_n m) ⊂ s0).
+    rewrite <-double_twice in *.
+    replace s0 with (trace_proj zero (Trace_lt NS3T n)) by (rewrite <-Heqt; trivial).
+    eapply subset_trans; [| apply sub_trace_proj; apply Trace_lt_sub; apply Hmn ].
+    apply set_subset_weaken; apply set_eq_symm; apply NS3Tl_precise.
+    
+    assert (s1 ⊂ (z_to_n p)).
+    replace (4 * p) with (double (double p)) in * by (simpl; unfold double; nliamega).
+    replace s1 with (trace_proj one (Trace_lt NS3T n)) by (rewrite <-Heqt; trivial).
+    eapply subset_trans.
+    apply sub_trace_proj.
+    apply (@Trace_lt_sub (TSum TNat (TSum TNat TNat)) )with (n := double (double p)); nliamega.
+    apply set_subset_weaken.
+    apply NS3Tr_precise.
+    
+    intros Hcontra.
+    eapply z_to_n_nosub; [apply Hpn|].
+    repeat (eapply subset_trans; [eassumption|]); apply subset_refl.
+  Qed.
+End NaiveSum3Unfair.
+
+Section PairFair.
+  Definition E_PairNN := (E_Pair (E_Trace zero E_Nat) (E_Trace one E_Nat)).
+  Lemma Pair_layer {tyl tyr} (e1: Enum tyl) (e2: Enum tyr) n
+  : Trace_from_to (E_Pair e1 e2) (n * n) (S n * S n)
+                  ≡ (Trace_lt e1 (S n)) ⊔ (Trace_lt e2 (S n)).
+  Proof.
+    apply trace_eq_eq'_equiv; split.
+    (* trace (e1 x e2) n^2 (n+1)^2 < (trace ) *)
+    (* TODO: come at this hard with some Ltac *)
+    - apply sub_trace_In_equiv; intros x tg Hin;
+      rewrite set_In_Trace_from_to in Hin by nliamega; destruct Hin as [k [[Hnnk HkSnSn] Hin]];
+      unfold Trace_on in Hin;
+      destruct (Enumerates_from_dec (E_Pair e1 e2) k) as [[v t] Henum]; simpl in Hin;
+      invert_Enumerates; subst;
+      destruct (sub_trace_In_equiv (lt ⊔ rt)
+                                   ((Trace_lt e1 (S n)) ⊔ (Trace_lt e2 (S n))));
+      apply H; [| assumption];
+      clear H H0;
+      apply sub_trace_plus_cong;
+      eapply Trace_lt_Enumerates; [| eassumption | | eassumption];
+      destruct (Pairing_bound ln rn k n); auto.
+    - eapply sub_trace_trans; [|apply trace_eq_weakenl; apply sub_trace_plus_eq; apply sub_trace_refl];
+      apply sub_trace_plus_cong.
+      (* trace e1 0..n+1 < trace (e1 x e2) n^2 (n+1)^2 *)
+      + apply sub_trace_In_equiv; intros x tg Hin;
+        rewrite set_In_Trace_lt in Hin by nliamega;
+        destruct Hin as [k [Hkn Hin]];
+        apply set_In_Trace_from_to; [nliamega|];
+        destruct (le_lt_dec n k);
+        [exists (k*k + k + n) | exists (k + n * n)];
+        (split; [nliamega|]);
+        unfold Trace_on; destruct (Enumerates_from_dec _ _) as [[v t] Henum]; simpl;
+        invert_Enumerates;
+        rewrite trace_proj_plus_distrl; apply set_union_intro1;
+        [ assert (Pairing (k * k + k + n) k n) by (constructor; nliamega)
+        | assert (Pairing (k + n * n) k n) by (constructor; nliamega)];
+        rewrite_pairing_to_fun; get_trace_ons; subst; auto.
+      + apply sub_trace_In_equiv; intros x tg Hin;
+        rewrite set_In_Trace_lt in Hin by nliamega;
+        destruct Hin as [k [Hkn Hin]];
+        apply set_In_Trace_from_to; [nliamega|];
+        destruct (le_lt_dec k n);
+        [exists (n * n + n + k) | exists (n + k * k)]; (split; [nliamega|]);
+        unfold Trace_on; destruct (Enumerates_from_dec _ _) as [[v t] Henum]; simpl;
+        invert_Enumerates;
+        rewrite trace_proj_plus_distrl; apply set_union_intro2;
+        [ assert (Pairing (n * n + n + k) n k) by (constructor; nliamega)
+        | assert (Pairing (n + k * k) n k) by (constructor; nliamega) ];
+        rewrite_pairing_to_fun; get_trace_ons; subst; auto.
+  Qed.
+
+  Lemma PairNN_layer :
+    forall n,
+      Trace_from_to E_PairNN (n * n) (S n * S n)
+      ≡ Tracing (z_to_n (S n)) (z_to_n (S n)) ∅ ∅.
+  Proof.
+    intros n.
+    eapply trace_eq_trans.
+    unfold E_PairNN; apply Pair_layer.
+    apply trace_eq_symm.
+    apply trace_eq_trans with ((Tracing (z_to_n (S n)) ∅ ∅ ∅)
+                                 ⊔ (Tracing ∅ (z_to_n (S n)) ∅ ∅)).
+    remember (S n) as k; unfold trace_plus; split4; auto; apply set_eq_symm; apply set_union_unitl.
+    apply trace_plus_cong; rewrite trace_proj_reconstruct.
+    split4; [ apply trace_lt_Nat | | | ]; rewrite trace_lt_Nat_off by discriminate; auto.
+    split4; [ | apply trace_lt_Nat | | ]; rewrite trace_lt_Nat_off by discriminate; auto.
+  Qed.      
+
+  Lemma Pair_precise
+  : forall n {ty1 ty2} e1 e2,
+      (Trace_lt (@E_Pair ty1 ty2 e1 e2) (n * n)) ≡ ((Trace_lt e1 n) ⊔ (Trace_lt e2 n)).
+    intros n.
+    induction n as [| n IHn]; [  intros; compute; tauto| ].
+    intros.
+    eapply trace_eq_trans.
+    apply trace_from_to_0_split with (m := n * n) (n := S n * S n); nliamega.
+    eapply trace_eq_trans; [apply sub_trace_plus_eq| apply Pair_layer].
+    eapply sub_trace_trans; [| apply trace_eq_weakenl; apply trace_eq_symm; apply Pair_layer ].
+    eapply sub_trace_trans; [apply trace_eq_weakenl; apply IHn|].
+    apply sub_trace_plus_cong; apply Trace_lt_sub; nliamega.
+  Qed.
+
+  Lemma PairPair_precise
+  : forall {ty1 ty2 ty3} n e1 e2 e3,
+      Trace_lt (@E_Pair ty1 _ e1 (@E_Pair ty2 ty3 e2 e3)) ((n * n) * (n * n))
+               ≡ (Trace_lt e1 (n * n)) ⊔ ((Trace_lt e2 n) ⊔ (Trace_lt e3 n)).
+  Proof.
+    intros.
+    eapply trace_eq_trans; [apply Pair_precise|].
+    apply trace_plus_cong; [apply trace_eq_refl| ].
+    apply Pair_precise.
+  Qed.
+
+  Lemma Pair_Fair_precise :
+    forall n, Trace_lt E_PairNN (n * n) ≡ Tracing (z_to_n n) (z_to_n n) ∅ ∅.
+  Proof.
+    induction n.
+    compute; tauto.
+    apply trace_eq_trans
+    with (t2 := ((Trace_lt E_PairNN (n * n)) ⊔ (Trace_from_to E_PairNN (n * n) (S n * S n)))).
+    apply trace_from_to_0_split; nliamega.
+    apply trace_eq_trans with (t2 := ((Tracing (z_to_n n) (z_to_n n) ∅ ∅)
+                                        ⊔ (Tracing (z_to_n (S n)) (z_to_n (S n)) ∅ ∅))).
+    apply trace_plus_cong; auto.
+    apply PairNN_layer.
+    apply trace_eq_trans with (t2 := (Tracing (z_to_n (S n)) (z_to_n (S n))) ∅ ∅).
+    unfold trace_eq.
+    split4;
+      [ (apply subset_union_eq; unfold z_to_n at 2; fold z_to_n; apply set_subset_add; apply subset_refl)
+      | (apply subset_union_eq; unfold z_to_n at 2; fold z_to_n; apply set_subset_add; apply subset_refl)
+      | apply set_eq_refl
+      | apply set_eq_refl ].
+
+    apply trace_eq_refl.
+  Qed.
+
+  Theorem PairFair : Fair2 (@E_Pair).
+    unfold Fair2.
+    intros n.
+    exists ((S n) * (S n)).
+
+    fold E_PairNN.
+    remember (Trace_lt E_PairNN (S n * S n)) as t.
+    destruct t as [t0 t1 t2 t3].
+    split; [nliamega|].
+    remember (Pair_Fair_precise (S n)) as Hteq; clear HeqHteq.
+    unfold trace_eq in Hteq.
+    remember (Trace_lt E_PairNN (S n * S n)) as t'.
+    destruct t'.
+    inversion Heqt; subst s s0.
+    destruct4 Hteq.
+    eapply set_eq_trans; [| apply set_eq_symm]; eauto.
+  Qed.
+End PairFair.
+
+Section NaiveTripleUnfair.
+
+  Definition NaiveTriple3 {ty1 ty2 ty3} e1 e2 e3 :=
+    @E_Pair ty1 _ e1 (@E_Pair ty2 ty3 e2 e3).
+
+  Definition traceNP3 := Trace_lt (NaiveTriple3 (E_Trace zero E_Nat) (E_Trace one E_Nat) (E_Trace two E_Nat)).
+
+  Definition NP3T := NaiveTriple3 (E_Trace zero E_Nat) (E_Trace one E_Nat) (E_Trace two E_Nat).
+
+  Theorem NaiveTripleUnfair : ~ (Fair3 (@NaiveTriple3)).
+  Proof.
+    apply AltUnfair3Suff.
+    unfold AltUnfair3.
+    fold NP3T.
+    exists 15.
+    intros n H.
+    assert (16 <= n) as H' by nliamega ; clear H.
+    remember (Trace_lt NP3T n) as t; destruct t as [t0 t1 t2 t3].
+    destruct (sqrt_4th_root_spread n) as [m [p [[Hmn Hnp] Hppmm]]]; auto.
+
+    left.
+    assert (~ t0 ⊂ t1); [ | intros []; contradiction].
+
+    assert ((z_to_n m) ⊂ t0).
+    - remember (Trace_lt NP3T (m * m)) as t; destruct t as [mm0 mm1 mm2 mm3].
+      assert ((Trace_lt NP3T (m * m)) ⊏ (Trace_lt NP3T n))
+        by (apply Trace_lt_sub; auto).
+      unfold sub_trace in H.
+      rewrite <-Heqt in H.
+      rewrite <-Heqt0 in H.
+      destruct4 H.
+      eapply subset_trans; try eassumption.
+      clear H H0 H1 H2; clear dependent t0; clear t1 t2 t3.
+      unfold NP3T, NaiveTriple3 in *.
+      remember (Pair_precise m (E_Trace zero E_Nat) (E_Pair (E_Trace one E_Nat) (E_Trace two E_Nat))).
+      clear Heqt.
+      rewrite <-Heqt0 in t.
+      remember (((Trace_lt (E_Trace zero E_Nat) m) ⊔ (Trace_lt (E_Pair (E_Trace one E_Nat) (E_Trace two E_Nat)) m))).
+      destruct t0.
+      replace mm0 with (trace_proj zero (Tracing mm0 mm1 mm2 mm3)) by auto.
+      eapply subset_trans; [| apply trace_eq_proj;  eassumption].
+      rewrite Heqt1.
+      rewrite trace_proj_plus_distrl.
+      apply subset_union_transl.
+      apply trace_lt_Nat.
+
+    - assert (t1 ⊂ (z_to_n p)).
+      remember (Trace_lt NP3T ((p * p) * (p * p))) as p4t.
+      assert ((Trace_lt NP3T n) ⊏ p4t) by (subst; apply Trace_lt_sub; auto; nliamega).
+      destruct p4t as [pt0 pt1 pt2 pt3].
+      unfold sub_trace in H0.
+      rewrite <-Heqt in H0.
+      destruct4 H0.
+      eapply subset_trans; try eassumption.
+      clear H0 H1 H2 H3; clear dependent t0; clear t1 t2 t3; clear dependent m; clear dependent n.
+      unfold NP3T in Heqp4t.
+      unfold NaiveTriple3 in Heqp4t.
+      remember (PairPair_precise p (E_Trace zero E_Nat) (E_Trace one E_Nat) (E_Trace two E_Nat)).
+      clear Heqt.
+      rewrite <-Heqp4t in t.
+      apply set_subset_weaken.
+      replace pt1 with (trace_proj one (Tracing pt0 pt1 pt2 pt3)) by trivial.
+      clear Heqp4t.
+      eapply set_eq_trans.
+      apply trace_eq_proj.
+      apply t.
+      apply set_eq_symm.
+      eapply set_eq_trans.
+      apply trace_lt_Nat with (tg := one).
+      rewrite trace_proj_plus_distrl.
+      rewrite trace_proj_plus_distrl.
+      rewrite trace_lt_Nat_off with (tg2 := zero); [| discriminate].
+      rewrite trace_lt_Nat_off with (tg2 := two); [| discriminate].
+      apply set_eq_symm.
+      eapply set_eq_trans; [apply set_union_unitl|].
+      eapply set_eq_trans; [apply set_union_unitr|].
+      apply set_eq_refl.
+
+      intros Hsub01.
+      eapply z_to_n_nosub; [apply Hppmm|].
+      repeat (eapply subset_trans; try eassumption); apply subset_refl.
+  Qed.
+End NaiveTripleUnfair.
