model/Pairing.v
@@ -1,0 +1,250 @@
+Require Import Coq.Numbers.Natural.Peano.NPeano.
+Require Import Coq.Arith.Arith_base.
+Require Import Psatz.
+
+Require Import Util.
+Inductive Pairing : nat -> nat -> nat -> Prop :=
+| P_XBig :
+    forall x y,
+      y <= x ->
+      Pairing (x*x + x + y) x y
+| P_XSmall :
+    forall x y,
+      x < y ->
+      Pairing (x + y*y) x y.
+Hint Constructors Pairing.
+
+Theorem Pairing_lt :
+  forall m n p,
+    Pairing p m n -> (m = 0 /\ n <= 1) \/ (m <= 1 /\ n = 0) \/ (p > m /\ p > n).
+Proof.
+  intros m n p P.
+  inversion P; subst; nliamega.
+Qed.
+
+Theorem Pairing_from_fun :
+  forall l r n1 n2,
+    Pairing n1 l r ->
+    Pairing n2 l r ->
+    n1 = n2.
+Proof.
+  intros l r n1 n2 P1 P2.
+  inversion P1; inversion P2; subst; nliamega.
+Qed.
+
+Lemma Pairing_to_incompat:
+  forall l1 l2 r1 r2,
+    r1 <= l1 ->
+    l2 < r2 ->
+    l2 + r2 * r2 = l1 * l1 + l1 + r1 ->
+    False.
+Proof.
+  intros; destruct (eq_nat_dec r2 l1); subst; nliamega.
+Qed.
+
+Theorem Pairing_to_fun :
+  forall n l1 l2 r1 r2,
+    Pairing n l1 r1 ->
+    Pairing n l2 r2 ->
+    (l1 = l2) /\ (r1 = r2).
+Proof.
+  intros n l1 l2 r1 r2 P1 P2.
+  inversion P1; inversion P2; clear P1; clear P2; subst.
+
+  replace l1 with l2 in * by nliamega.
+  replace r1 with r2 in * by nliamega.
+  auto.
+
+  cut False. contradiction.
+  eapply (Pairing_to_incompat _ _ _ _ H H3 H4).
+
+  cut False. contradiction.
+  symmetry in H4.
+  eapply (Pairing_to_incompat _ _ _ _ H3 H H4).
+
+  replace r1 with r2 in * by nliamega.
+  replace l1 with l2 in * by nliamega.
+  auto.
+Qed.
+
+Theorem Pairing_to_l_fun :
+  forall n l1 l2 r1 r2,
+    Pairing n l1 r1 ->
+    Pairing n l2 r2 ->
+    l1 = l2.
+Proof.
+  intros n l1 l2 r1 r2 P1 P2.
+  edestruct (Pairing_to_fun _ _ _ _ _ P1 P2). auto.
+Qed.
+Theorem Pairing_to_r_fun :
+  forall n l1 l2 r1 r2,
+    Pairing n l1 r1 ->
+    Pairing n l2 r2 ->
+    r1 = r2.
+Proof.
+  intros n l1 l2 r1 r2 P1 P2.
+  edestruct (Pairing_to_fun _ _ _ _ _ P1 P2). auto.
+Qed.
+
+Theorem Pairing_to_dec:
+  forall x y,
+    { n | Pairing n x y }.
+Proof.
+  intros x y.
+  destruct (le_lt_dec y x) as [BIG | SMALL]; eauto.
+Defined.
+
+Definition Pairing_to x y : nat := proj1_sig (Pairing_to_dec x y).
+Corollary Pairing_to_sound :
+  forall l r,
+    Pairing (Pairing_to l r) l r.
+Proof.
+  intros l r. unfold Pairing_to.
+  remember (Pairing_to_dec l r) as vn.
+  destruct vn as [n P]. simpl. auto.
+Qed.
+Hint Resolve Pairing_to_sound.
+
+(* sqrt lemmas *)
+Lemma sqrt_lemma z : (z - (sqrt z * sqrt z)) - sqrt z <= sqrt z.
+Proof.
+  destruct (sqrt_spec z); nliamega.
+Qed.
+
+Lemma sqrt_lemma' z :
+  (z - (sqrt z) * (sqrt z) < (sqrt z))
+  -> z = z - (sqrt z * sqrt z) + (sqrt z * sqrt z).
+Proof.
+  remember (sqrt_spec z); nliamega.
+Qed.
+
+Lemma sqrt_lemma'' k n :
+  (n * n <= k < S n * S n) -> k - sqrt k * sqrt k - sqrt k < S n.
+Proof.
+  intros H; rewrite (Nat.sqrt_unique k n); lia.
+Qed.
+
+Lemma sqrt_slower_than_id n :
+  4 <= n ->
+  (S (sqrt (S n))) < n.
+Proof.
+  intros H4n.
+  remember (n - 4) as k.
+  replace n with (4 + k) by nliamega.
+  clear dependent n.
+  rename k into n.
+  induction n.
+  compute; reflexivity.
+  assert (sqrt (S (4 + S n)) <= (S (S (S n)))); [| nliamega].
+  eapply le_trans; [apply Nat.sqrt_succ_le|].
+  replace (4 + S n) with (S (4 + n)) by nliamega.
+  nliamega.
+Qed.
+
+Lemma sqrt_4th_root_spread n :
+  16 <= n ->
+  exists m p,
+    m * m <= n < (p * p) * (p * p) /\ p < m.
+Proof.
+  intros H.
+  exists (S (S (sqrt (S (sqrt n))))).
+  exists (S (sqrt (S (sqrt n)))).
+  split; [| nliamega].
+  split; [| destruct (sqrt_spec n); destruct (sqrt_spec (S (sqrt n))); nliamega ].
+  destruct (sqrt_spec n).
+  apply le_trans with (m := sqrt n * sqrt n); auto.
+  assert (S (S (sqrt (S (sqrt n)))) <= sqrt n) as Hperf; [|(apply mult_le_compat; apply Hperf)].
+  assert (4 <= sqrt n).
+  replace 4 with (sqrt 16) .
+  apply Nat.sqrt_le_mono; auto.
+  compute; trivial.
+  apply sqrt_slower_than_id; auto.
+Qed.
+
+Lemma nat_le_iff : forall m p, (forall q : nat, q <= m -> q <= p) <-> m <= p.
+Proof.
+  split.
+  intros H. apply (H m); auto.
+  intros H q; nliamega.
+Qed.
+
+Lemma nat_lt_iff : forall m p, (forall q : nat, q < m -> q < p) <-> m <= p.
+Proof.
+  destruct m.
+  intros p; split; [nliamega| intros _ q contra; inversion contra].
+  destruct p.
+  split.
+  intros contra; assert (m < 0) by (apply contra; auto); nliamega.
+  intros contra; inversion contra.
+  split.
+  intros H.
+  assert (m <= p); [| nliamega].
+  apply nat_le_iff.
+  intros q Hqm.
+  assert (q < S p); [| nliamega].
+  apply H; nliamega.
+  intros; nliamega.
+Qed.
+
+Theorem Pairing_from_dec:
+  forall n,
+    { xy | Pairing n (fst xy) (snd xy) }.
+Proof.
+  (* (z - rootz^2, rootz)          if z - rootz^2 <  rootz
+     (rootz, (z - rootz^2) -rootz) if z - rootz^2 >= rootz
+   *)
+  intros z.
+  remember (sqrt z) as rootz.
+  destruct (le_lt_dec rootz (z - (rootz * rootz))).
+  (* P_XBig, x >= y: x*x + x + y *)
+  exists (rootz, (z - rootz * rootz) - rootz).
+  assert (z = rootz * rootz + rootz + ((z - rootz * rootz) - rootz)) by nliamega.
+  assert (((z - (rootz * rootz)) - rootz) = z - (rootz * rootz + rootz)) by nliamega.
+
+  rewrite H at 1.
+  constructor 1.
+  simpl.
+
+  remember (sqrt_spec z).
+  rewrite Heqrootz in *.
+  apply sqrt_lemma.
+
+  (* P_XSmall: x < y: x + y*y *)
+  exists (z - (rootz * rootz), rootz).
+  subst.
+  rewrite sqrt_lemma' at 1; [| auto].
+  simpl; constructor 2; auto.
+Defined.
+
+Definition Pairing_from n : (nat * nat) := proj1_sig (Pairing_from_dec n).
+Corollary Pairing_from_sound :
+  forall n l r,
+    (l, r) = Pairing_from n ->
+    Pairing n l r.
+Proof.
+  intros n l r. unfold Pairing_from.
+  remember (Pairing_from_dec n) as vlr.
+  destruct vlr as [[l' r'] P]. simpl in *.
+  intros EQ. congruence.
+Qed.
+Hint Resolve Pairing_from_sound.
+
+Theorem Pairing_bound l r k n
+: k < S n * S n 
+  -> Pairing k l r
+  -> l < S n /\ r < S n.
+Proof.
+  intros H Hp; inversion Hp; subst; nliamega.
+Qed.
+
+Ltac rewrite_pairing_to_fun :=
+  match goal with
+    | [ H1 : Pairing ?x ?y1 ?z1, H2 : Pairing ?x ?y2 ?z2 |- _ ] =>
+      destruct (Pairing_to_fun _ _ _ _ _ H1 H2) as [Hl Hr]; rewrite Hl in *; rewrite Hr in *; clear H1 H2 Hl Hr
+  end.
+
+Ltac rewrite_pairing_from_fun :=
+  match goal with
+    | [ H1: Pairing ?n1 ?l ?r, H2: Pairing ?n2 ?l ?r |- _ ] =>
+      erewrite (Pairing_from_fun _ _ _ _ H1 H2) in *; clear H1 H2
+  end.
