model/Trace.v
@@ -1,0 +1,232 @@
+Require Import Sets Util.
+
+Inductive Trace :=
+| Tracing : set' -> set' -> set' -> set' -> Trace.
+
+Inductive tag : Set :=
+| zero  : tag
+| one   : tag
+| two   : tag
+| three : tag.
+
+Definition trace_proj tg t :=
+  match t with
+    | Tracing t0 t1 t2 t3 =>
+      match tg with
+        | zero  => t0
+        | one   => t1
+        | two   => t2
+        | three => t3
+      end
+  end.
+
+Definition trace_zero : Trace := Tracing ∅ ∅ ∅ ∅.
+                                         Notation ε := trace_zero.
+Definition trace_plus (t1 t2 : Trace) : Trace :=
+  match (t1, t2) with
+    | (Tracing l1 l2 l3 l4, Tracing r1 r2 r3 r4) =>
+      Tracing (l1 ∪ r1) (l2 ∪ r2) (l3 ∪ r3) (l4 ∪ r4)
+  end.
+Notation "x ⊔ y" := (trace_plus x y) (at level 50).
+
+Definition trace_one n t : Trace :=
+  match t with
+    | zero  => Tracing (set_add' n ∅) ∅ ∅ ∅
+    | one   => Tracing ∅ (set_add' n ∅) ∅ ∅
+    | two   => Tracing ∅ ∅ (set_add' n ∅) ∅
+    | three => Tracing ∅ ∅ ∅ (set_add' n ∅)
+  end.
+
+Definition trace_eq (t1 t2 : Trace) : Prop :=
+  match (t1, t2) with
+    | (Tracing l0 l1 l2 l3, Tracing r0 r1 r2 r3) =>
+      l0 ≃ r0 /\ l1 ≃ r1 /\ l2 ≃ r2 /\ l3 ≃ r3
+  end.
+Notation "t1 ≡ t2" := (trace_eq t1 t2) (at level 70, no associativity).
+
+Definition sub_trace (t1 t2 : Trace) : Prop :=
+  match (t1, t2) with
+    | (Tracing l0 l1 l2 l3, Tracing r0 r1 r2 r3) =>
+      l0 ⊂ r0 /\ l1 ⊂ r1 /\ l2 ⊂ r2 /\ l3 ⊂ r3
+  end.
+Notation "t1 ⊏ t2" := (sub_trace t1 t2) (at level 70, no associativity).
+
+Theorem sub_trace_refl t : t ⊏ t.
+Proof.
+  unfold sub_trace; destruct t; split4; apply subset_refl.
+Qed.
+Hint Resolve sub_trace_refl.
+
+Theorem sub_trace_trans t1 t2 t3 : t1 ⊏ t2 -> t2 ⊏ t3 -> t1 ⊏ t3.
+Proof.
+  unfold sub_trace; destruct t1, t2, t3.
+  intros H1 H2; destruct4 H1; destruct4 H2.
+  split4; eapply subset_trans; eauto.
+Qed.
+
+Theorem sub_trace_zero t : ε ⊏ t.
+Proof. destruct t; compute; tauto. Qed.
+
+Theorem trace_eq_proj t1 t2 tg : t1 ≡ t2 -> (trace_proj tg t1) ≃ (trace_proj tg t2).
+Proof.
+  unfold trace_eq, trace_proj; destruct t1; destruct t2; destruct tg; intuition.
+Qed.
+
+Theorem sub_trace_proj t1 t2 tg : t1 ⊏ t2 -> (trace_proj tg t1) ⊂ (trace_proj tg t2).
+Proof.
+  unfold sub_trace; destruct t1; destruct t2; destruct tg; intuition.
+Qed.
+
+Definition trace_eq' t1 t2 : Prop :=
+  t1 ⊏ t2 /\ t2 ⊏ t1.
+Theorem trace_eq'_weakenl t1 t2 : trace_eq' t1 t2 -> t1 ⊏ t2.
+Proof. unfold trace_eq'; intuition. Qed.
+Theorem trace_eq'_weakenr t1 t2 : trace_eq' t1 t2 -> t2 ⊏ t1.
+Proof. unfold trace_eq'; intuition. Qed.
+Theorem trace_eq_eq'_equiv t1 t2 : t1 ≡ t2 <-> trace_eq' t1 t2.
+Proof.
+  unfold trace_eq, trace_eq', sub_trace, set_eq;
+  destruct t1; destruct t2; intuition.
+Qed.
+
+Theorem trace_eq_weakenl t1 t2 : t1 ≡ t2 -> t1 ⊏ t2.
+Proof. rewrite trace_eq_eq'_equiv; apply trace_eq'_weakenl. Qed.
+
+Theorem trace_eq_weakenr t1 t2 : t1 ≡ t2 -> t2 ⊏ t1.
+Proof. rewrite trace_eq_eq'_equiv; apply trace_eq'_weakenr. Qed.
+
+Theorem trace_plus_cong t1 t2 t3 t4 : t1 ≡ t3 -> t2 ≡ t4 -> (t1 ⊔ t2) ≡ (t3 ⊔ t4).
+  unfold trace_eq.
+  destruct t1; destruct t2; destruct t3; destruct t4.
+  unfold trace_plus.
+  intros H; destruct4 H.
+  intros H'; destruct4 H'.
+  split4; apply set_union_cong; auto.
+Qed.
+
+Theorem trace_eq_refl t : t ≡ t.
+Proof.
+  unfold trace_eq; destruct t; split4; apply set_eq_refl.
+Qed.
+Hint Resolve trace_eq_refl.
+
+Theorem trace_eq_symm t1 t2 : t1 ≡ t2 -> t2 ≡ t1.
+Proof.
+  unfold trace_eq.
+  destruct t1; destruct t2.
+  intros H; destruct4 H.
+  split4; apply set_eq_symm; auto.
+Qed.
+
+Theorem trace_eq_trans t1 t2 t3 : t1 ≡ t2 -> t2 ≡ t3 -> t1 ≡ t3.
+Proof.
+  unfold trace_eq.
+  destruct t1; destruct t2; destruct t3.
+  intros H; destruct4 H.
+  intros H'; destruct4 H'.
+  split4; eapply set_eq_trans; eauto.
+Qed.
+
+Theorem trace_plus_comm t1 t2 : (t1 ⊔ t2) ≡ (t2 ⊔ t1).
+Proof.
+  destruct t1, t2.
+  unfold trace_plus.
+  split4; apply set_eq_union_comm.
+Qed.
+
+Theorem trace_plus_assoc t1 t2 t3 : (t1 ⊔ (t2 ⊔ t3)) ≡ ((t1 ⊔ t2) ⊔ t3).
+Proof.
+  destruct t1, t2, t3.
+  unfold trace_plus.
+  split4; apply set_eq_symm; apply set_union_assoc.
+Qed.
+
+Theorem sub_trace_plus_transl t tl tr
+: t ⊏ tl -> t ⊏ (tl ⊔ tr).
+Proof.
+  intros H; destruct t; destruct tl; destruct tr;
+  destruct4 H; split4; apply subset_union_transl; auto.
+Qed.
+
+Theorem sub_trace_plus_transr t tl tr
+: t ⊏ tr -> t ⊏ (tl ⊔ tr).
+Proof.
+  intros H.
+  eapply sub_trace_trans.
+  Focus 2.
+  apply trace_eq_weakenl.
+  apply trace_plus_comm.
+  apply sub_trace_plus_transl; auto.
+Qed.
+
+Theorem sub_trace_plus_eq : forall t1 t2, t1 ⊏ t2 -> (t1 ⊔ t2) ≡ t2.
+Proof.
+  intros t1 t2 H; destruct t1; destruct t2;
+  destruct4 H; split4; apply subset_union_eq; auto.
+Qed.
+
+Theorem trace_plus_unitl t : (ε ⊔ t) ≡ t.
+Proof.
+  destruct t; split4; apply set_union_unitl.
+Qed.
+
+Theorem trace_plus_unitl_gen t1 t2 : t1 ≡ t2 -> (ε ⊔ t1) ≡ t2.
+Proof.
+  intros H.
+  eapply trace_eq_trans; [ apply trace_plus_unitl | auto].
+Qed.
+
+
+Theorem trace_plus_unitr t :
+  (t ⊔ ε) ≡ t.
+Proof.
+  eapply trace_eq_trans;
+  [apply trace_plus_comm| apply trace_plus_unitl].
+Qed.
+
+
+Theorem trace_plus_unitr_gen t1 t2 : t1 ≡ t2 -> (t1 ⊔ ε) ≡ t2.
+Proof.
+  intros H.
+  eapply trace_eq_trans; [ apply trace_plus_unitr | auto].
+Qed.
+
+Theorem sub_trace_plus_cong tl1 tr1 tl2 tr2 : 
+  tl1 ⊏ tl2
+  -> tr1 ⊏ tr2
+  -> (tl1 ⊔ tr1) ⊏ (tl2 ⊔ tr2).
+Proof.
+  unfold sub_trace, trace_plus.
+  destruct tl1; destruct tl2; destruct tr1; destruct tr2.
+  intros Hl; destruct4 Hl.
+  intros Hr; destruct4 Hr.
+  split4; apply set_union_subset_cong; auto.
+Qed.
+
+Theorem trace_proj_reconstruct t 
+: t = Tracing (trace_proj zero t) (trace_proj one t) (trace_proj two t) (trace_proj three t).
+Proof.
+  destruct t; reflexivity.
+Qed.
+
+Theorem sub_trace_In_equiv t1 t2
+: t1 ⊏ t2 
+  <-> 
+  (forall x tg, x ∈ (trace_proj tg t1) -> x ∈ (trace_proj tg t2)).
+Proof.
+  destruct t1; destruct t2; split.
+  intros Hst x tg Hin; destruct4 Hst; destruct tg; eapply subset_In; eassumption.
+  intros H; rewrite trace_proj_reconstruct; rewrite trace_proj_reconstruct at 1;
+  split4; apply subset_In_def; intros; apply H; assumption.
+Qed.
+
+Theorem sub_trace_In_util t1 t2 x tg
+: t1 ⊏ t2 
+  -> x ∈ (trace_proj tg t1)
+  -> x ∈ (trace_proj tg t2).
+Proof.
+  intros Hsub.
+  generalize x tg.
+  generalize Hsub.
+  apply sub_trace_In_equiv.
+Qed.
