model/Util.v
@@ -1,0 +1,45 @@
+Require Import Coq.Logic.Eqdep_dec.
+Require Import Omega.
+Require Import Psatz.
+
+Ltac nliamega := try omega; try lia; try nia; fail "omega, lia and nia all failed".
+
+(* Turn hypotheses of shape (existT h1 h2 l = existT h1 h2 r) into l = r if equality on lhs is decidable *)
+Ltac dec_K :=
+  match goal with
+    | [ H : existT ?P ?L ?x = existT ?P ?L ?y |- _ ] => apply inj_pair2_eq_dec in H;
+        [subst |]; auto
+  end.
+
+(* Try possible contradictions *)
+Ltac mycontra :=
+  match goal with
+    | [ H: context[_ -> False] |- False ] =>
+      eapply H; eauto; fail
+  end.
+
+(* sumbool notation a la cpdt *)
+Notation Yes := (left _).
+Notation No := (right _).
+Notation "l &&& r" := (if l then r else No) (at level 70).
+Notation Refine x := (if x then Yes else No).
+
+(* sumor notation a la cpdt *)
+Notation "{{ x }}" := (exist _ x _).
+
+Ltac sumbool_contra :=
+  match goal with
+    | [ H: inl _ = inr _ |- _ ] => inversion H
+    | [ H: inr _ = inl _ |- _ ] => inversion H
+  end.
+
+Ltac destruct_eq :=
+  match goal with
+    | [ H: (?x1, ?y1) = (?x2, ?y2) |- _ ] =>
+      (assert (x1 = x2) by congruence); (assert (y1 = y2) by congruence); subst; clear H
+    | [ H: inl ?x = inl ?y |- _ ] => (assert (x = y) by congruence); subst; clear H
+    | [ H: inr ?x = inr ?y |- _ ] => (assert (x = y) by congruence); subst; clear H
+  end.
+
+Ltac split4 := split; [| split; [| split]].
+Ltac destruct4 H := destruct H as [? [? [? ?]]].
